cava/Cava/Arrow/DeriveSpec.v
@@ -21,8 +21,17 @@ Require Import Cava.Arrow.ArrowExport.
 (* This file contains tactics and notations designed to simplify proofs that
    derive or prove specifications for kappa-level circuits. *)
 
+(* convenient notation *)
+Notation kinterp x := (interp_combinational' (x coq_func)).
+Notation minterp x := (interp_combinational' ((module_body x) coq_func)).
+
+Lemma kinterp_via_minterp {x y} {f: Module (Kappa x y)} {s} {X}:
+  minterp f X = s
+  -> kinterp (instantiate f) X = s.
+Proof. destruct f. intuition. Qed.
+
 Ltac kappa_spec_begin :=
-  intros; cbn [interp_combinational'];
+  intros; cbn [interp_combinational' module_body];
   repeat match goal with
          | |- context [primitive_semantics ?p] =>
            let x := constr:(primitive_semantics p) in
@@ -38,6 +47,7 @@ Ltac kappa_spec_step :=
   match goal with
   | _ => progress autorewrite with kappa_interp
   | H : context [interp_combinational' (_ coq_func) _ = _] |- _ => rewrite H by eauto
+  | H: minterp ?f _ = _ |- _ => apply kinterp_via_minterp in H
   | |- context [interp_combinational'] => kappa_spec_begin
   end.
 Ltac kappa_spec := kappa_spec_begin; repeat kappa_spec_step.
@@ -93,7 +103,4 @@ Ltac derive_foldl_spec :=
       erewrite (fold_left_ext f g) by derive_spec
     end
   end.
-
-(* convenient notation *)
-Notation kinterp x := (interp_combinational' (x coq_func)).
 
